libcrux-intrinsics/proofs/fstar/extraction/Libcrux_intrinsics.Avx2_extract.fsti
@@ -39,7 +39,13 @@ val mm256_storeu_si256_i32 (output: t_Slice i32) (vector: t_Vec256)
     : Prims.Pure (t_Slice i32) Prims.l_True (fun _ -> Prims.l_True)
 
 val mm_storeu_si128 (output: t_Slice i16) (vector: t_Vec128)
-    : Prims.Pure (t_Slice i16) Prims.l_True (fun _ -> Prims.l_True)
+    : Prims.Pure (t_Slice i16)
+      (requires (Core.Slice.impl__len #i16 output <: usize) >=. mk_usize 8)
+      (ensures
+        fun output_future ->
+          let output_future:t_Slice i16 = output_future in
+          (Core.Slice.impl__len #i16 output_future <: usize) =.
+          (Core.Slice.impl__len #i16 output <: usize))
 
 val mm_storeu_si128_i32 (output: t_Slice i32) (vector: t_Vec128)
     : Prims.Pure (t_Slice i32) Prims.l_True (fun _ -> Prims.l_True)
@@ -160,7 +166,13 @@ val mm_mullo_epi16 (lhs rhs: t_Vec128)
           vec128_as_i16x8 result ==
           Spec.Utils.map2 mul_mod (vec128_as_i16x8 lhs) (vec128_as_i16x8 rhs))
 
-val mm256_cmpgt_epi16 (lhs rhs: t_Vec256) : Prims.Pure t_Vec256 Prims.l_True (fun _ -> Prims.l_True)
+val mm256_cmpgt_epi16 (lhs rhs: t_Vec256)
+    : Prims.Pure t_Vec256
+      Prims.l_True
+      (ensures
+        fun result ->
+          let result:t_Vec256 = result in
+          forall i. i % 16 >= 1 ==> result i == 0)
 
 val mm256_cmpgt_epi32 (lhs rhs: t_Vec256) : Prims.Pure t_Vec256 Prims.l_True (fun _ -> Prims.l_True)
 
